example/Bellman_Ford.thy
@@ -1,7 +1,7 @@
 theory Bellman_Ford
-  imports "../DP_Lifting"
+  imports "../DP_Lifting" "../DP_Consistency"
 begin
-
+  
 consts n :: nat
 consts W :: "nat \<Rightarrow> nat \<Rightarrow> int"
 term 0 (**)
@@ -12,7 +12,7 @@ fun bf :: "nat\<times>nat \<Rightarrow> int" where
 | "bf (Suc k, j) = fold min [bf (k, i) + W i j. i \<leftarrow> [0..<n]] (bf (k, j))"
 term 0 (**)
 *)
-
+  
 fun bf :: "nat\<times>nat \<Rightarrow> int" where
   "bf (0, j) = W 0 j"
 | "bf (Suc k, j) =
@@ -24,7 +24,7 @@ fun bf :: "nat\<times>nat \<Rightarrow> int" where
       (bf (k, j))"
 thm bf.simps
 term 0 (**)
-
+  
 fun bf\<^sub>T :: "nat\<times>nat \<Rightarrow>\<^sub>T int" where
   "bf\<^sub>T$ (0, j) =CHECKMEM= \<langle>W 0 j\<rangle>"
 | "bf\<^sub>T$ (Suc k, j) =CHECKMEM=
@@ -32,7 +32,34 @@ fun bf\<^sub>T :: "nat\<times>nat \<Rightarrow>\<^sub>T int" where
     . \<langle>min\<^sub>T\<rangle>
     . (\<langle>map\<^sub>T\<rangle>
       . \<langle>\<lambda>i. \<langle>plus\<^sub>T\<rangle> . (bf\<^sub>T (k, i)) . \<langle>W i j\<rangle>\<rangle>
-      . \<langle>upt 0 n\<rangle>)
+      . (\<langle>upt\<^sub>T\<rangle> . \<langle>0\<rangle> . \<langle>n\<rangle>))
     . (bf\<^sub>T (k, j))"
 term 0 (**)
+  
+interpretation dp: dp_consistency bf .
+context
+  includes lifting_syntax
+begin
+lemma "dp.consistentDP bf\<^sub>T"
+  apply (rule dp.consistentDP_intro, induct_tac rule: bf\<^sub>T.induct, unfold bf\<^sub>T.simps; rule dp.consistentS_checkmem, unfold bf.simps)
+  subgoal by transfer_prover
+  subgoal premises prems
+    thm prems
+    supply [transfer_rule] = prems
+    apply transfer_prover_start
+                        apply transfer_step
+                        apply transfer_step
+                        apply transfer_step
+                        apply transfer_step
+                        apply transfer_step
+                        apply transfer_step
+                        apply transfer_step
+                        apply transfer_step
+                        apply transfer_step
+                        apply transfer_step
+                        apply transfer_step
+                        apply transfer_step
+      (* going wrong here *)
+      (* bf\<^sub>T (Pair k i) should be proved directly by prems(1) rather than be separated *)
+    oops
 end
